Dafny/examples/demoChallengeProb1.i.dfy
@@ -2,7 +2,7 @@ include "../llvm.i.dfy"
 include "../control_flow.i.dfy"
 include "generalInstructions.i.dfy"
 include "../types.dfy"
-include "../memory.dfy"
+include "../memory.i.dfy"
 
 module demo_challenge_prob_1 {
     import opened LLVM_def
@@ -18,6 +18,21 @@ module demo_challenge_prob_1 {
 //####################################################################
 
 /*
+
+int main(int argc, const char *argv[]) {
+  // default input
+  unsigned char buf[8] = { 0, 1, 2, 3, 4, 5, 6, 7};
+
+  // optional input
+  for(int i = 1; i < argc && i < sizeof(buf)/sizeof(buf[0]); i++) {
+    buf[i] = (unsigned char)atoi(argv[i]);
+  }
+
+  rx_message_routine(buf);
+  return 0;
+}
+
+
 void rx_message_routine(unsigned char buf[]){
   // buf[3] is the integer value, 0-255km, buff[2] is the decimal
   uint16_t speed_value = (buf[3] << 8) + buf[2];  // <-------- Vulnerability here
@@ -61,181 +76,219 @@ define void @rx_message_routine(i8* nocapture readonly %0) local_unnamed_addr #0
   %11 = load i8, i8* %10, align 1
   %12 = zext i8 %11 to i32
   %13 = add nsw i32 %8, %12
-  %14 = trunc i32 %13 to i16
-  %16 = zext i16 %14 to i32
-  %17 = icmp sgt i32 %16, 0
+  %17 = icmp eq i32 %13, 0 // ugt
   ret void
 }
 */
 
-function {:opaque} demo_challenge_prob_1_code(dst:lvm_operand_opr,s:MemState,op1:lvm_operand_opr,op2:lvm_operand_opr,
-                                              var_5:lvm_operand_opr,var_index2:lvm_operand_opr,comp:lvm_operand_opr):lvm_code
+function {:opaque} demo_challenge_prob_1_code(speed_value:lvm_operand_opr,s:MemState,var_0:lvm_operand_opr,
+                                              var_5:lvm_operand_opr,var_10:lvm_operand_opr,var_17:lvm_operand_opr,
+                                              var_6:lvm_operand_opr,var_7:lvm_operand_opr,var_8:lvm_operand_opr,var_11:lvm_operand_opr,var_12:lvm_operand_opr):lvm_code
 {
     reveal_IntFits();
     var index3 := D(Int(3,IntType(8,false)));
     var index2 := D(Int(2,IntType(8,false)));
     var shl_amount := D(Int(8,IntType(1,false)));
 
-    var var_6:lvm_operand_opr :| var_6 == dst;
-    var var_7:lvm_operand_opr :| var_7 == dst;
-    var var_8:lvm_operand_opr :| var_8 == dst;
 
-    lvm_Block(lvm_CCons(Ins(GETELEMENTPTR(var_5,1,op1,index3)),                  // %5 = getelementptr inbounds i8, i8* %0, i64 3
-              lvm_CCons(Ins(LOAD(var_6,s,1,var_5)),                              // %6 = load i8, i8* %2, align 1, !tbaa !4
-              lvm_CCons(Ins(ZEXT(var_7,1,var_6,4)),                              // %7 = zext i8 %3 to i32
-              lvm_CCons(Ins(SHL(var_8,var_7,shl_amount)),                        // %8 = shl i32 %7, 8
-              lvm_CCons(Ins(GETELEMENTPTR(var_index2,1,op2,index2)),             // %10 = getelementptr inbounds i8, i8* %0, i64 2
-              lvm_CCons(Ins(LOAD(var_index2,s,1,var_index2)),                    // %11 = load i8, i8* %10, align 1
-              lvm_CCons(Ins(ZEXT(var_index2,1,var_index2,4)),                    // %12 = zext i8 %11 to i32
-              lvm_CCons(Ins(ADD(dst,4,var_8,var_index2)),                        // %13 = add nsw i32 %8, %12
-              lvm_CCons(Ins(ICMP(comp,sgt,4,var_8,D(Int(0,IntType(4,false))))),  // %17 = icmp sgt i32 %16, 0 
-              lvm_CCons(Ins(RET(D(Void))),lvm_CNil())))))))))))                     // ret void
+    lvm_Block(lvm_CCons(Ins(GETELEMENTPTR(var_5,1,var_0,index3)),                         // %5 = getelementptr inbounds i8, i8* %0, i64 3
+              lvm_CCons(Ins(LOAD(var_6,s,1,var_5)),                                       // %6 = load i8, i8* %2, align 1, !tbaa !4
+              lvm_CCons(Ins(ZEXT(var_7,1,var_6,4)),                                       // %7 = zext i8 %3 to i32
+              lvm_CCons(Ins(SHL(var_8,var_7,shl_amount)),                                 // %8 = shl i32 %7, 8
+              lvm_CCons(Ins(GETELEMENTPTR(var_10,1,var_0,index2)),                        // %10 = getelementptr inbounds i8, i8* %0, i64 2
+              lvm_CCons(Ins(LOAD(var_11,s,1,var_10)),                                     // %11 = load i8, i8* %10, align 1
+              lvm_CCons(Ins(ZEXT(var_12,1,var_11,4)),                                     // %12 = zext i8 %11 to i32
+              lvm_CCons(Ins(ADD(speed_value,4,var_8,var_12)),                             // %13 = add nsw i32 %8, %12
+              lvm_CCons(Ins(ICMP(var_17,ugt,4,speed_value,D(Int(0,IntType(4,false))))),   // %17 = icmp eq i32 %13, 0 
+              lvm_CCons(Ins(RET(D(Void))),lvm_CNil())))))))))))                           // ret void
 
 }
 
-lemma lvm_demo_challenge_prob_1(lvm_b0:lvm_codes, lvm_s0:lvm_state, lvm_sN:lvm_state, 
-            dst:lvm_operand_opr,op1:lvm_operand_opr,op2:lvm_operand_opr,
-            var_5:lvm_operand_opr,var_index2:lvm_operand_opr,comp:lvm_operand_opr)
-  returns (lvm_bM:lvm_codes, lvm_sM:lvm_state)
-  requires op1.D?;
-  requires op2.D?;
-  requires lvm_require(lvm_b0, demo_challenge_prob_1_code(dst,lvm_s0.m,op1,op2,var_5,var_index2,comp), lvm_s0, lvm_sN)
-  requires lvm_is_dst_opr(dst, lvm_s0)
-  requires lvm_is_src_opr(op1, lvm_s0)
-  requires lvm_get_ok(lvm_s0)
+lemma lvm_demo_simple_challenge_prob_1(lvm_b0:lvm_codes, lvm_s0:lvm_state,var_0:lvm_operand_opr,var_5:lvm_operand_opr,
+                                       var_6:lvm_operand_opr,var_7:lvm_operand_opr,var_8:lvm_operand_opr,var_10:lvm_operand_opr,
+                                       var_11:lvm_operand_opr,var_12:lvm_operand_opr,speed_value:lvm_operand_opr, var_17:lvm_operand_opr)
+      returns (lvm_bM:lvm_codes, lvm_sM:lvm_state,lvm_sMs:seq<lvm_state>)
+// PRE Conditions 
+  requires exists sN :: lvm_require(lvm_b0, demo_challenge_prob_1_code(speed_value,lvm_s0.m,var_0,var_5,var_10,var_17,var_6,var_7,var_8,var_11,var_12), lvm_s0, sN)
+  requires lvm_b0.tl.CNil?
 
-  requires ValidOperand(lvm_s0,op1);
-  requires ValidOperand(lvm_s0,op2);
-  requires ValidOperand(lvm_s0,dst);
+  requires ValidState(lvm_s0)
+  requires ValidOperand(lvm_s0,var_0);
   requires ValidOperand(lvm_s0,var_5);
-  requires ValidOperand(lvm_s0,var_index2);
-  requires ValidOperand(lvm_s0,comp);
-  requires operandsUnique(lvm_s0,[dst,var_index2,var_5,comp]);
-
-  requires OperandContents(lvm_s0,op1).Ptr?;
-  requires OperandContents(lvm_s0,op2).Ptr?;
-  requires OperandContents(lvm_s0,op1).bid in lvm_s0.m.mem; //needed for IsValidBid for valid input
-  requires OperandContents(lvm_s0,op2).bid in lvm_s0.m.mem; //needed for IsValidBid for valid input
-  requires IsValidBid(lvm_s0.m,op1.d.bid) ==> op1.d.offset + ((Int(3,IntType(8,false))).val * 1) < |lvm_s0.m.mem[op1.d.bid]|;
-  requires IsValidBid(lvm_s0.m,op2.d.bid) ==> op2.d.offset + ((Int(2,IntType(8,false))).val * 1) < |lvm_s0.m.mem[op2.d.bid]|;
-
-//   
-
-  ensures ValidOperand(lvm_sM,dst)
-  ensures ValidOperand(lvm_sM, var_index2)
-  ensures lvm_get_ok(lvm_sM)
-
-  ensures  !OperandContents(lvm_sM, dst).Void? ==> OperandContents(lvm_sM, dst).Int?;
-  ensures  !OperandContents(lvm_sM, dst).Void? ==> OperandContents(lvm_sM, dst).itype.size == 4;
-  ensures  !OperandContents(lvm_sM, dst).Void? ==> OperandContents(lvm_sM, dst).val < 0x1_0000_0000;
-  ensures  !OperandContents(lvm_sM, dst).Void? ==> OperandContents(lvm_sM, dst).val >= 0;
-
-  ensures  (!OperandContents(lvm_sM, dst).Void? && !OperandContents(lvm_sM, var_index2).Void?) ==> lvm_state_eq(lvm_sM, lvm_update_ok(lvm_sM, lvm_update_mem( lvm_sM, lvm_s0)))
-  ensures  (!OperandContents(lvm_sM, dst).Void? && !OperandContents(lvm_sM, var_index2).Void?) ==> lvm_ensure(lvm_b0, lvm_bM, lvm_s0, lvm_sM, lvm_sN)
-
-{
-  reveal_demo_challenge_prob_1_code();
-  reveal_lvm_code_Ret();
-  reveal_lvm_LOAD();
-  reveal_lvm_code_Add();
-  reveal_lvm_code_ZEXT();
-  reveal_lvm_code_SHL();
-  reveal_lvm_code_ICMP();
-  reveal_lvm_code_Empty();
-  reveal_lvm_code_GetElementPtr();
-  reveal_ValidData();
-  reveal_evalCodeOpaque();
-  reveal_eval_code();
-  var operands :=[dst,var_index2,var_5,comp];
-  var var_7:lvm_operand_opr :| var_7 == dst;
-  var var_8:lvm_operand_opr :| var_8 == dst;
-
-  assert demo_challenge_prob_1_code(dst,lvm_s0.m,op1,op2,var_5,var_index2,comp).Block?;
-  assert lvm_b0.hd.Block?;
-  assert evalBlock(lvm_b0, lvm_s0, lvm_sN);
-
-  ghost var lvm_ltmp1, lvm_cM:lvm_code, lvm_ltmp2 := lvm_lemma_block(lvm_b0, lvm_s0, lvm_sN);
-  lvm_sM := lvm_ltmp1;
-  lvm_bM := lvm_ltmp2;
-  var lvm_b1:lvm_codes := lvm_get_block(lvm_cM);
-
-  assert lvm_b1.hd == Ins(GETELEMENTPTR(var_5,1,op1,D(Int(3,IntType(8,false)))));
-  assert lvm_sM == lvm_s0;
-
-  ghost var lvm_b2, lvm_s2 := lvm_lemma_GetElementPtr(lvm_b1, lvm_s0, lvm_sM, var_5, lvm_s0.m,1,op1,D(Int(3,IntType(8,false))));
-  assert lvm_s0.m == lvm_s2.m;
-  assert StateNext(lvm_s0,lvm_s2);
-
-  ghost var lvm_b3, lvm_s3 := lvm_lemma_Load(lvm_b2, lvm_s2, lvm_sM, dst,1,var_5);
-  assert lvm_s3.m == lvm_s2.m;
-  assert StateNext(lvm_s2,lvm_s3);
-
-  if (OperandContents(lvm_s3,dst).Void?) { // LOAD ins failed
-    lvm_sM := lvm_s3;
-    assert OperandContents(lvm_sM, dst).Void?;
-    return;
-  }
-  ghost var lvm_b4, lvm_s4 := lvm_lemma_Zext(lvm_b3, lvm_s3, lvm_sM, var_7, 1,dst,4);
-  assert lvm_s3.m == lvm_s4.m;
-  assert StateNext(lvm_s3,lvm_s4);
-
-  var shl_amount := D(Int(8,IntType(1,false)));
-  ghost var lvm_b5, lvm_s5 := lvm_lemma_Shl(lvm_b4, lvm_s4, lvm_sM, var_8,var_7,shl_amount);
-  assert lvm_s4.m == lvm_s5.m;
-  assert StateNext(lvm_s4,lvm_s5);
-
-
-  assert OperandContents(lvm_s5,var_8).itype.size == 4;
-  assert OperandContents(lvm_s5, var_8).val >= 0;
-  assert OperandContents(lvm_s5,var_8).Int?;
-
-  assert lvm_b5.hd.Ins?;
-  assert lvm_b5.hd.ins.GETELEMENTPTR?;
-
-  ghost var lvm_b6, lvm_s6 := lvm_lemma_GetElementPtr(lvm_b5, lvm_s5, lvm_sM, var_index2, lvm_s5.m,1,op2,D(Int(2,IntType(8,false))));
-  assert lvm_s5.m == lvm_s6.m;
-  assert StateNext(lvm_s5,lvm_s6);
-
-    // LOAD now
-  ghost var lvm_b7, lvm_s7 := lvm_lemma_Load(lvm_b6, lvm_s6, lvm_sM, var_index2,1,var_index2);
-  assert lvm_s6.m == lvm_s7.m;
-  assert StateNext(lvm_s6,lvm_s7);
-  if (OperandContents(lvm_s7,var_index2).Void?) { // LOAD ins failed
-    lvm_sM := lvm_s7;
-    assert OperandContents(lvm_sM, var_index2).Void?;
-    return;
-  }
+  requires ValidOperand(lvm_s0,var_6);
+  requires ValidOperand(lvm_s0,var_7);
+  requires ValidOperand(lvm_s0,var_8);
+  requires ValidOperand(lvm_s0,var_11);
+  requires ValidOperand(lvm_s0,var_12);
+  requires ValidOperand(lvm_s0,speed_value);
+  requires ValidOperand(lvm_s0,var_10);
+  requires ValidOperand(lvm_s0,var_17);
+  requires operandsUnique(lvm_s0,[speed_value,var_10,var_5,var_6,var_7,var_8,var_11,var_12,var_17]);
   
-  assert lvm_b7.hd.ins.ZEXT?;
-  ghost var lvm_b8, lvm_s8 := lvm_lemma_Zext(lvm_b7, lvm_s7, lvm_sM, var_index2, 1,var_index2,4);
-  assert StateNext(lvm_s7,lvm_s8);
+  requires var_0.D? && OperandContents(lvm_s0,var_0).Ptr?;
+  requires OperandContents(lvm_s0,var_0).bid in lvm_s0.m.mem; //needed for IsValidBid for valid input
+  requires IsValidBid(lvm_s0.m,var_0.d.bid) ==> var_0.d.offset + ((Int(8,IntType(1,false))).val * 1) < |lvm_s0.m.mem[var_0.d.bid]|;
 
-  assert lvm_b8.hd.ins.ADD?;
-  ghost var lvm_b9, lvm_s9 := lvm_lemma_Add(lvm_b8, lvm_s8, lvm_sM, dst,4,dst,var_index2);
-  assert StateNext(lvm_s8,lvm_s9);
+// POST Conditions
+  // end state is valid 
+  ensures ValidState(lvm_sM)
+  // operands are valid in end state
+  ensures ValidOperand(lvm_sM,var_0);
+  ensures ValidOperand(lvm_sM,var_5);
+  ensures ValidOperand(lvm_sM,var_6);
+  ensures ValidOperand(lvm_sM,var_7);
+  ensures ValidOperand(lvm_sM,var_8);
+  ensures ValidOperand(lvm_sM,var_11);
+  ensures ValidOperand(lvm_s0,var_12);
+  ensures ValidOperand(lvm_sM,speed_value);
+  ensures ValidOperand(lvm_sM,var_10);
+  ensures ValidOperand(lvm_sM,var_17);
 
-  assert operandsUnique(lvm_s9,operands);
-  assert operands[0] == dst && operands[1] == var_index2;
-  assert OperandContents(lvm_s9,var_8).Int?;
-
-  ghost var lvm_b10, lvm_s10:= lvm_lemma_Icmp(lvm_b9, lvm_s9, lvm_sM, comp,sgt,4,var_8,D(Int(0,IntType(4,false))));
-  assert StateNext(lvm_s9,lvm_s10);
-
-  ghost var lvm_b11, lvm_s11:= lvm_lemma_Ret(lvm_b10, lvm_s10, lvm_sM, dst, D(Void));
-  assert StateNext(lvm_s10,lvm_s11);
-
-  assert lvm_b11 == (lvm_CNil());
-  assert eval_code(lvm_Block(lvm_b11), lvm_s10, lvm_sM);
-  lvm_sM := lvm_lemma_empty(lvm_s11,lvm_sM);
-  assert OperandContents(lvm_sM, dst).Int?;
-  assert OperandContents(lvm_sM,dst).itype.size == 4;
-  assert OperandContents(lvm_sM,dst).itype.size >= 4;
-
-  assert ValidState(lvm_sM);
-  assert StateNext(lvm_s11,lvm_sM);
-
+  ensures  (!OperandContents(lvm_sM, var_6).Void? && !OperandContents(lvm_sM, var_11).Void?) 
+               ==> OperandContents(lvm_sM, var_8).Int?;
+  ensures  (!OperandContents(lvm_sM, var_6).Void? && !OperandContents(lvm_sM, var_11).Void?) 
+              ==> OperandContents(lvm_sM, speed_value).Int?;
+  ensures  (!OperandContents(lvm_sM, var_6).Void? && !OperandContents(lvm_sM, var_11).Void?) 
+              ==> OperandContents(lvm_sM, var_17).Int?;
+  ensures  (!OperandContents(lvm_sM, var_6).Void? && !OperandContents(lvm_sM, var_11).Void?) 
+              ==> OperandContents(lvm_sM, speed_value).itype.size == 4;
+  ensures  (!OperandContents(lvm_sM, var_6).Void? && !OperandContents(lvm_sM, var_11).Void?) 
+             ==> OperandContents(lvm_sM, speed_value).val < 0x1_0000_0000;
+  ensures  (!OperandContents(lvm_sM, var_6).Void? && !OperandContents(lvm_sM, var_11).Void?) 
+             ==> OperandContents(lvm_sM, speed_value).val >= 0;
   
-}
+  ensures  (!OperandContents(lvm_sM, var_6).Void? && !OperandContents(lvm_sM, var_11).Void?) 
+              ==> (OperandContents(lvm_sM,speed_value).val > 0 ==> OperandContents(lvm_sM,var_17).val == 1);
 
+  ensures  (!OperandContents(lvm_sM, var_6).Void? && !OperandContents(lvm_sM, var_11).Void?) ==> lvm_ensure(lvm_b0, lvm_CNil(), lvm_s0, lvm_sM, lvm_sM)
+  ensures ValidStateSeq(lvm_sMs);
+  {
+    reveal_demo_challenge_prob_1_code();
+    reveal_lvm_code_Ret();
+    reveal_lvm_LOAD();
+    reveal_lvm_code_Add();
+    reveal_lvm_code_ZEXT();
+    reveal_lvm_code_SHL();
+    reveal_lvm_code_ICMP();
+    reveal_lvm_code_Empty();
+    reveal_lvm_code_GetElementPtr();
+    reveal_ValidData();
+    reveal_evalCodeOpaque();
+    reveal_eval_code();
+    lvm_sMs := [lvm_s0];
+    var operands :=[speed_value,var_10,var_5,var_6,var_7,var_8,var_11,var_12,var_17];
+
+    var codeBlock := demo_challenge_prob_1_code(speed_value,lvm_s0.m,var_0,var_5,var_10,var_17,var_6,var_7,var_8,var_11,var_12);
+    var sN :|  lvm_require(lvm_b0, codeBlock, lvm_s0, sN);
+
+    ghost var lvm_ltmp1, lvm_cM:lvm_code, lvm_ltmp2 := lvm_lemma_block(lvm_b0, lvm_s0, sN);
+    lvm_sM := lvm_ltmp1;
+    lvm_bM := lvm_ltmp2;
+    assert lvm_bM == lvm_b0.tl;
+    assert lvm_bM.CNil?;
+    var lvm_b1:lvm_codes := lvm_get_block(lvm_cM);
+
+    assert lvm_b1.hd == Ins(GETELEMENTPTR(var_5,1,var_0,D(Int(3,IntType(8,false)))));
+    assert lvm_sM == lvm_s0;
+
+    ghost var lvm_b2, lvm_s2 := lvm_lemma_GetElementPtr(lvm_b1, lvm_s0, lvm_sM, var_5, lvm_s0.m,1,var_0,D(Int(3,IntType(8,false))));
+    assert lvm_s0.m == lvm_s2.m;
+    assert StateNext(lvm_s0,lvm_s2);
+    lvm_sMs := lvm_sMs + [lvm_s2];
+
+    ghost var lvm_b3, lvm_s3 := lvm_lemma_Load(lvm_b2, lvm_s2, lvm_sM, var_6,1,var_5);
+    assert lvm_s3.m == lvm_s2.m;
+    assert StateNext(lvm_s2,lvm_s3);
+    lvm_sMs := lvm_sMs + [lvm_s3];
+
+
+    if (OperandContents(lvm_s3,var_6).Void?) { // LOAD ins failed
+      lvm_sM := lvm_s3;
+      assert OperandContents(lvm_sM, var_6).Void?;
+      return;
+    }
+
+    ghost var lvm_b4, lvm_s4 := lvm_lemma_Zext(lvm_b3, lvm_s3, lvm_sM, var_7, 1,var_6,4);
+    assert lvm_s3.m == lvm_s4.m;
+    assert StateNext(lvm_s3,lvm_s4);
+    lvm_sMs := lvm_sMs + [lvm_s4];
+
+    assert OperandContents(lvm_s4,var_7).Int?;
+    assert OperandContents(lvm_s4,var_7).itype.size == 4;
+
+
+    var shl_amount := D(Int(8,IntType(1,false)));
+    ghost var lvm_b5, lvm_s5 := lvm_lemma_Shl(lvm_b4, lvm_s4, lvm_sM, var_8,var_7,shl_amount);
+    assert lvm_s4.m == lvm_s5.m;
+    assert StateNext(lvm_s4,lvm_s5);
+    lvm_sMs := lvm_sMs + [lvm_s5];
+
+
+    assert OperandContents(lvm_s5,var_8).itype.size == 4;
+    assert OperandContents(lvm_s5, var_8).val >= 0;
+    assert OperandContents(lvm_s5,var_8).Int?;
+    assert !OperandContents(lvm_s5,var_8).itype.signed;
+
+    assert lvm_b5.hd.Ins?;
+    assert lvm_b5.hd.ins.GETELEMENTPTR?;
+
+    ghost var lvm_b6, lvm_s6 := lvm_lemma_GetElementPtr(lvm_b5, lvm_s5, lvm_sM, var_10, lvm_s5.m,1,var_0,D(Int(2,IntType(8,false))));
+    assert lvm_s5.m == lvm_s6.m;
+    assert StateNext(lvm_s5,lvm_s6);
+    lvm_sMs := lvm_sMs + [lvm_s6];
+
+      // LOAD now
+    assert operandsUnique(lvm_s6,operands);
+    assert operands[5] == var_8 && operands[1] == var_10;
+    assert OperandContents(lvm_s6,var_8).Int?;
+    assert !OperandContents(lvm_s6,var_8).itype.signed;
+
+    ghost var lvm_b7, lvm_s7 := lvm_lemma_Load(lvm_b6, lvm_s6, lvm_sM, var_11,1,var_10);
+    assert lvm_s6.m == lvm_s7.m;
+    assert StateNext(lvm_s6,lvm_s7);
+    lvm_sMs := lvm_sMs + [lvm_s7];
+    if (OperandContents(lvm_s7,var_11).Void?) { // LOAD ins failed
+      lvm_sM := lvm_s7;
+      assert OperandContents(lvm_sM, var_11).Void?;
+      return;
+    }
+    assert operandsUnique(lvm_s6,operands);
+    assert operands[5] == var_8 && operands[6] == var_11;
+
+    assert lvm_b7.hd.ins.ZEXT?;
+    ghost var lvm_b8, lvm_s8 := lvm_lemma_Zext(lvm_b7, lvm_s7, lvm_sM, var_12, 1,var_11,4);
+    assert StateNext(lvm_s7,lvm_s8);
+    lvm_sMs := lvm_sMs + [lvm_s8];
+
+    assert lvm_b8.hd.ins.ADD?;
+    ghost var lvm_b9, lvm_s9 := lvm_lemma_Add(lvm_b8, lvm_s8, lvm_sM, speed_value,4,var_8,var_12);
+    assert StateNext(lvm_s8,lvm_s9);
+    lvm_sMs := lvm_sMs + [lvm_s9];
+
+    assert operandsUnique(lvm_s9,operands);
+    assert operands[0] == speed_value && operands[1] == var_10;
+    assert OperandContents(lvm_s9,speed_value).Int?;
+    assert OperandContents(lvm_s9,speed_value).itype.size == 4;
+
+    ghost var lvm_b10, lvm_s10:= lvm_lemma_Icmp(lvm_b9, lvm_s9, lvm_sM, var_17,ugt,4,speed_value,D(Int(0,IntType(4,false))));
+    assert StateNext(lvm_s9,lvm_s10);
+    lvm_sMs := lvm_sMs + [lvm_s10];
+    assert OperandContents(lvm_s10,var_17).Int?;
+    assert !OperandContents(lvm_s10,var_17).itype.signed;
+    assert OperandContents(lvm_s10,var_17).itype.size == 1;
+    assert OperandContents(lvm_s9,speed_value).val > 0 ==> OperandContents(lvm_s10,var_17).val == 1;
+
+    ghost var lvm_b11, lvm_s11:= lvm_lemma_Ret(lvm_b10, lvm_s10, lvm_sM, speed_value, D(Void));
+    assert StateNext(lvm_s10,lvm_s11);
+    lvm_sMs := lvm_sMs + [lvm_s11];
+
+    assert lvm_b11 == (lvm_CNil());
+    assert eval_code(lvm_Block(lvm_b11), lvm_s10, lvm_sM);
+    lvm_sM := lvm_lemma_empty(lvm_s11,lvm_sM);
+    assert ValidState(lvm_sM);
+    assert StateNext(lvm_s11,lvm_sM);
+    lvm_sMs := lvm_sMs + [lvm_sM];
+  
+  }
 
 }
