Dafny/Operations/binaryOperationsHelper.i.dfy
@@ -14,14 +14,17 @@ module binary_operations_helper_i {
         requires v0.itype.size == 1
         ensures out.Int?
         ensures validBitWidth(out.itype.size)
+        ensures out.itype.size == 1
+        ensures !out.itype.signed
         ensures (!v0.itype.signed) ==> out.val == (v0.val + v1.val) % 0x100
         ensures (v0.itype.signed) ==> ToTwosComp(out).val == (v0.val + v1.val) % 0x100
         
         {
             reveal_ToTwosComp();
             reveal_FromTwosComp();
-            if (!v0.itype.signed) then UInt8(BitwiseAdd8(DataToUInt8(ToTwosComp(v0)),DataToUInt8(ToTwosComp(v1)))) else 
-                                       FromTwosComp(UInt8(BitwiseAdd8(DataToUInt8(ToTwosComp(v1)),DataToUInt8(ToTwosComp(v0)))))  
+            UInt8(BitwiseAdd8(DataToUInt8(ToTwosComp(v0)),DataToUInt8(ToTwosComp(v1)))) 
+            // if (!v0.itype.signed) then UInt8(BitwiseAdd8(DataToUInt8(ToTwosComp(v0)),DataToUInt8(ToTwosComp(v1)))) else 
+            //                            FromTwosComp(UInt8(BitwiseAdd8(DataToUInt8(ToTwosComp(v1)),DataToUInt8(ToTwosComp(v0)))))  
         }
         
     function evalADD16(size:nat,v0:Data,v1:Data):  (out:Data)
@@ -32,14 +35,15 @@ module binary_operations_helper_i {
         requires v0.itype.size == 2
         ensures out.Int?
         ensures validBitWidth(out.itype.size)
+        ensures out.itype.size == 2
+        ensures !out.itype.signed
         ensures (!v0.itype.signed) ==> out.val == (v0.val + v1.val) % 0x10000
         ensures (v0.itype.signed) ==> ToTwosComp(out).val == (v0.val + v1.val) % 0x10000
         
         {
             reveal_ToTwosComp();
             reveal_FromTwosComp();
-            if (!v0.itype.signed) then UInt16(BitwiseAdd16(DataToUInt16(ToTwosComp(v0)),DataToUInt16(ToTwosComp(v1)))) else 
-                                       FromTwosComp(UInt16(BitwiseAdd16(DataToUInt16(ToTwosComp(v1)),DataToUInt16(ToTwosComp(v0)))))
+            UInt16(BitwiseAdd16(DataToUInt16(ToTwosComp(v0)),DataToUInt16(ToTwosComp(v1))))
         }
 
     function evalADD32(size:nat,v0:Data,v1:Data):  (out:Data)
@@ -50,14 +54,15 @@ module binary_operations_helper_i {
         requires v0.itype.size == 4
         ensures out.Int?
         ensures validBitWidth(out.itype.size)
+        ensures out.itype.size == 4
+        ensures !out.itype.signed
         ensures (!v0.itype.signed) ==> out.val == (v0.val + v1.val) % 0x1_0000_0000
         ensures (v0.itype.signed) ==> ToTwosComp(out).val == (v0.val + v1.val) % 0x1_0000_0000
         
         {
             reveal_ToTwosComp();
             reveal_FromTwosComp();
-            if (!v0.itype.signed) then UInt32(BitwiseAdd32(DataToUInt32(ToTwosComp(v0)),DataToUInt32(ToTwosComp(v1)))) else  
-                                       FromTwosComp(UInt32(BitwiseAdd32(DataToUInt32(ToTwosComp(v1)),DataToUInt32(ToTwosComp(v0)))))
+            UInt32(BitwiseAdd32(DataToUInt32(ToTwosComp(v0)),DataToUInt32(ToTwosComp(v1)))) 
         }
 
     function evalADD64(size:nat,v0:Data,v1:Data):  (out:Data)
@@ -68,14 +73,15 @@ module binary_operations_helper_i {
         requires v0.itype.size == 8
         ensures out.Int?
         ensures validBitWidth(out.itype.size)
+        ensures out.itype.size == 8
+        ensures !out.itype.signed
         ensures (!v0.itype.signed) ==> out.val == (v0.val + v1.val) % 0x1_0000_0000_0000_0000
         ensures (v0.itype.signed) ==> ToTwosComp(out).val == (v0.val + v1.val) % 0x1_0000_0000_0000_0000
         
         {
             reveal_ToTwosComp();
             reveal_FromTwosComp();
-            if (!v0.itype.signed) then UInt64(BitwiseAdd64(DataToUInt64(ToTwosComp(v0)),DataToUInt64(ToTwosComp(v1)))) else  
-                                       FromTwosComp(UInt64(BitwiseAdd64(DataToUInt64(ToTwosComp(v1)),DataToUInt64(ToTwosComp(v0)))))
+            UInt64(BitwiseAdd64(DataToUInt64(ToTwosComp(v0)),DataToUInt64(ToTwosComp(v1))))
         }
 
     // SUB //
@@ -87,6 +93,7 @@ module binary_operations_helper_i {
         requires v0.itype.size == 1
         ensures out.Int?
         ensures validBitWidth(out.itype.size)
+        ensures out.itype.size == 1
         ensures  ToTwosComp(out).val == (v0.val - v1.val) % 0x100
         
         {
@@ -104,6 +111,7 @@ module binary_operations_helper_i {
         requires v0.itype.size == 2
         ensures out.Int?
         ensures validBitWidth(out.itype.size)
+        ensures out.itype.size == 2
         ensures  ToTwosComp(out).val == (v0.val - v1.val) % 0x10000
         
         {
@@ -121,6 +129,7 @@ module binary_operations_helper_i {
         requires v0.itype.size == 4
         ensures out.Int?
         ensures validBitWidth(out.itype.size)
+        ensures out.itype.size == 4
         ensures  ToTwosComp(out).val == (v0.val - v1.val) % 0x1_0000_0000
         
         {
@@ -138,6 +147,7 @@ module binary_operations_helper_i {
         requires v0.itype.size == 8
         ensures out.Int?
         ensures validBitWidth(out.itype.size)
+        ensures out.itype.size == 8
         ensures  ToTwosComp(out).val == (v0.val - v1.val) % 0x1_0000_0000_0000_0000
         
         {
