Dafny/examples/generalInstructions.i.dfy
@@ -1,7 +1,7 @@
 include "../llvm.i.dfy"
 include "../control_flow.i.dfy"
 include "../types.dfy"
-include "../memory.dfy"
+include "../memory.i.dfy"
 include "../Operations/binaryOperations.i.dfy"
 include "../Operations/conversionOperations.i.dfy"
 include "../Operations/bitwiseBinaryOperations.i.dfy"
@@ -36,13 +36,11 @@ lemma lvm_lemma_Add(lvm_b0:lvm_codes, lvm_s0:lvm_state, lvm_sN:lvm_state,
   requires ValidOperand(lvm_s0,src2);
   requires OperandContents(lvm_s0,src2).Int?;
   requires ValidOperand(lvm_s0,dst);
-  requires OperandContents(lvm_s0,dst).Int?;
+  // requires OperandContents(lvm_s0,dst).Int?;
 
-  requires ValidOperand(lvm_s0,dst);
   requires typesMatch(OperandContents(lvm_s0,src1),OperandContents(lvm_s0,src2))
-  requires OperandContents(lvm_s0,src2).Int?;
+  requires size == OperandContents(lvm_s0,src1).itype.size
   requires lvm_code_Add(dst, size,src1,src2).Ins?;
-  requires ValidOperand(lvm_s0,dst)
 // //   
   ensures  lvm_ensure(lvm_b0, lvm_bM, lvm_s0, lvm_sM, lvm_sN)
   ensures  lvm_get_ok(lvm_sM)
@@ -51,13 +49,18 @@ lemma lvm_lemma_Add(lvm_b0:lvm_codes, lvm_s0:lvm_state, lvm_sN:lvm_state,
   ensures OperandContents(lvm_sM,src1).Int?;
   ensures  ValidOperand(lvm_sM,src2)
   ensures OperandContents(lvm_sM,src2).Int?;
-  ensures typesMatch(OperandContents(lvm_sM,src1),OperandContents(lvm_sM,src2))
+  ensures OperandContents(lvm_sM,dst).Int?;
+  ensures OperandContents(lvm_sM,dst).itype.size == size;
+  ensures !OperandContents(lvm_sM,dst).itype.signed
+
 
   ensures  OperandContents(lvm_sM,dst).Int?;
   ensures  lvm_state_eq(lvm_sM, lvm_update_mem( lvm_sM, lvm_update_all(lvm_sM, lvm_s0)))
   ensures  lvm_state_eq(lvm_sM, lvm_update_ok(lvm_sM, lvm_update_all( lvm_sM, lvm_s0)))
   ensures  forall s2 :: evalCode(lvm_b0.hd, lvm_s0, s2) ==> s2.ok
-  ensures OperandContents(lvm_sM, dst).val == evalADD(OperandContents(lvm_s0,dst).itype.size,OperandContents(lvm_s0,src1),OperandContents(lvm_s0,src2)).val;
+    // ensures typesMatch(OperandContents(lvm_sM,src1),OperandContents(lvm_sM,src2))
+
+  // ensures OperandContents(lvm_sM, dst).val == evalADD(OperandContents(lvm_s0,dst).itype.size,OperandContents(lvm_s0,src1),OperandContents(lvm_s0,src2)).val;
   ensures ToTwosComp(OperandContents(lvm_sM, dst)).val == 
           (OperandContents(lvm_s0, src1).val + OperandContents(lvm_s0, src2).val) % Pow256(OperandContents(lvm_s0, src1).itype.size)
   ensures forall d :: ValidOperand(lvm_s0,d) && d != dst ==> ValidOperand(lvm_sM,d) && OperandContents(lvm_s0,d) == OperandContents(lvm_sM,d)
@@ -88,11 +91,11 @@ lemma lvm_lemma_Add(lvm_b0:lvm_codes, lvm_s0:lvm_state, lvm_sN:lvm_state,
     assert ValidState(lvm_sM);
     assert ValidOperand(lvm_sM,dst);
     assert evalIns(lvm_code_Add(dst, size,src1,src2).ins,lvm_s0,lvm_sM);
-    var evalA := evalADD(OperandContents(lvm_s0,dst).itype.size,OperandContents(lvm_s0,src1),OperandContents(lvm_s0,src2));
-    assert evalUpdate(lvm_s0, dst, evalA,lvm_sM);
+    // var evalA := evalADD(OperandContents(lvm_s0,dst).itype.size,OperandContents(lvm_s0,src1),OperandContents(lvm_s0,src2));
+    // assert evalUpdate(lvm_s0, dst, evalA,lvm_sM);
     assert (forall d :: ValidOperand(lvm_s0,d) && d != dst ==> ValidOperand(lvm_sM,d) && OperandContents(lvm_s0,d) == OperandContents(lvm_sM,d));
-    assert ValidData(lvm_sM,evalADD(OperandContents(lvm_s0,dst).itype.size,OperandContents(lvm_s0,src1),OperandContents(lvm_s0,src2)));
-    assert OperandContents(lvm_sM, dst).val == evalADD(OperandContents(lvm_s0,dst).itype.size,OperandContents(lvm_s0,src1),OperandContents(lvm_s0,src2)).val;
+    // assert ValidData(lvm_sM,evalADD(OperandContents(lvm_s0,dst).itype.size,OperandContents(lvm_s0,src1),OperandContents(lvm_s0,src2)));
+    assert OperandContents(lvm_sM, dst).val == evalADD(OperandContents(lvm_s0,src1).itype.size,OperandContents(lvm_s0,src1),OperandContents(lvm_s0,src2)).val;
     reveal_evalCodeOpaque();
 }
 
@@ -146,7 +149,7 @@ ensures lvm_s0.m == lvm_sM.m;
   lvm_bM := lvm_ltmp2;
 //   var lvm_b1:lvm_codes := lvm_get_block(lvm_cM);
   assert lvm_sM.ok;
-      assert lvm_b0.tl == lvm_bM;
+  assert lvm_b0.tl == lvm_bM;
 
   assert ValidState(lvm_sM);
   assert evalCode_lax(lvm_cM, lvm_s0, lvm_sM);
@@ -192,8 +195,7 @@ lemma lvm_lemma_Ret(lvm_b0:lvm_codes, lvm_s0:lvm_state, lvm_sN:lvm_state,dst:lvm
   ghost var lvm_ltmp1, lvm_cM:lvm_code, lvm_ltmp2 := lvm_lemma_block(lvm_b0, lvm_s0, lvm_sN);
   lvm_sM := lvm_ltmp1;
   lvm_bM := lvm_ltmp2;
-//   var lvm_b1:lvm_codes := lvm_get_block(lvm_cM);
-  // assert lvm_sM.ok;
+
   assert lvm_b0.tl == lvm_bM;
 
   assert ValidState(lvm_sM);
@@ -204,16 +206,13 @@ lemma lvm_lemma_Ret(lvm_b0:lvm_codes, lvm_s0:lvm_state, lvm_sN:lvm_state,dst:lvm
 
 function method{:opaque} lvm_LOAD(dst:lvm_operand_opr,s:MemState,t:bitWidth,op1:lvm_operand_opr):lvm_code
 {
-    //getelementptr
     reveal_IntFits();
     Ins(LOAD(dst,s,t,op1))
-
 }
 
 
 lemma lvm_lemma_Load(lvm_b0:lvm_codes, lvm_s0:lvm_state, lvm_sN:lvm_state,dst:lvm_operand_opr,t:bitWidth,op1:lvm_operand_opr)
   returns (lvm_bM:lvm_codes, lvm_sM:lvm_state)
-//   requires dst.LV?;
   requires lvm_require(lvm_b0, lvm_LOAD(dst,lvm_s0.m,t,op1), lvm_s0, lvm_sN)
   requires lvm_is_dst_opr(dst, lvm_s0)
   requires lvm_is_src_opr(op1, lvm_s0)
@@ -224,20 +223,18 @@ lemma lvm_lemma_Load(lvm_b0:lvm_codes, lvm_s0:lvm_state, lvm_sN:lvm_state,dst:lv
   requires OperandContents(lvm_s0,op1).Ptr?;
   requires MemValid(lvm_s0.m);
   requires IsValidPtr(lvm_s0.m,OperandContents(lvm_s0,op1).bid,OperandContents(lvm_s0,op1).offset);
-  requires lvm_s0.m == lvm_sN.m; // this is the issue
-//   requires exists d:Data :: Load(lvm_s0.m,lvm_sN.m,OperandContents(lvm_s0,op1).bid,OperandContents(lvm_s0,op1).offset,d);
-
+  requires lvm_s0.m == lvm_sN.m;
 //   
   ensures  lvm_ensure(lvm_b0, lvm_bM, lvm_s0, lvm_sM, lvm_sN)
   ensures  lvm_get_ok(lvm_sM)
-  ensures ValidOperand(lvm_sM,dst);
+  ensures  ValidOperand(lvm_sM,dst);
   ensures  !OperandContents(lvm_sM,dst).Ptr?;
   ensures  OperandContents(lvm_sM,dst).Int? || OperandContents(lvm_sM,dst).Void?;
 
   ensures OperandContents(lvm_sM,dst).Bytes? ==> validBitWidth(|OperandContents(lvm_sM,dst).bytes|)
   ensures OperandContents(lvm_sM,dst).Int? || OperandContents(lvm_sM,dst).Bytes? || OperandContents(lvm_sM,dst).Void?;
   ensures OperandContents(lvm_sM,dst).Int? ==> OperandContents(lvm_sM,dst).itype.size == t;
-  ensures  lvm_s0.m == lvm_sM.m;
+  ensures lvm_s0.m == lvm_sM.m;
   ensures forall d :: ValidOperand(lvm_s0,d) && d != dst ==> ValidOperand(lvm_sM,d) && OperandContents(lvm_s0,d) == OperandContents(lvm_sM,d)
   ensures StateNext(lvm_s0,lvm_sM)
 
@@ -275,9 +272,9 @@ lemma lvm_lemma_Load(lvm_b0:lvm_codes, lvm_s0:lvm_state, lvm_sN:lvm_state,dst:lv
 
   assert lvm_b0.tl == lvm_bM;
   assert !OperandContents(lvm_sM,dst).Ptr?;
-  assert OperandContents(lvm_sM,dst).Int? || OperandContents(lvm_sM,dst).Bytes? ||OperandContents(lvm_sM,dst).Void?;
-   assert OperandContents(lvm_sM,dst).Int? ==> OperandContents(lvm_sM,dst).itype.size == t;
-
+  assert OperandContents(lvm_sM,dst).Int? || OperandContents(lvm_sM,dst).Void?;
+  assert OperandContents(lvm_sM,dst).Int? ==> OperandContents(lvm_sM,dst).itype.size == t;
+  
   assert ValidState(lvm_sM);
   assert evalCode_lax(lvm_cM, lvm_s0, lvm_sM);
 }
@@ -300,13 +297,10 @@ lemma lvm_lemma_Zext(lvm_b0:lvm_codes, lvm_s0:lvm_state, lvm_sN:lvm_state,
   requires lvm_is_src_opr(op1, lvm_s0)
   requires lvm_get_ok(lvm_s0)
 
-//   requires ValidInstruction(lvm_s0, lvm_code_ZEXT(dst,t,op1,dstSize).ins);
   requires ValidOperand(lvm_s0,op1);
   requires ValidOperand(lvm_s0,dst);
   requires OperandContents(lvm_s0,op1).Int?;
-//   requires t == OperandContents(lvm_s0,op1).itype.size;
   requires OperandContents(lvm_s0,op1).itype.size < dstSize;
-  requires OperandContents(lvm_s0,dst).Int?;
 //   requires !OperandContents(lvm_s0,dst).itype.signed;
 
 // //   
@@ -367,7 +361,6 @@ lemma lvm_lemma_Sext(lvm_b0:lvm_codes, lvm_s0:lvm_state, lvm_sN:lvm_state,
   requires ValidOperand(lvm_s0,op1);
   requires ValidOperand(lvm_s0,dst);
   requires OperandContents(lvm_s0,op1).Int?;
-//   requires t == OperandContents(lvm_s0,op1).itype.size;
   requires OperandContents(lvm_s0,op1).itype.size < dstSize;
   requires OperandContents(lvm_s0,dst).Int?;
 //   requires !OperandContents(lvm_s0,dst).itype.signed;
@@ -400,12 +393,12 @@ lemma lvm_lemma_Sext(lvm_b0:lvm_codes, lvm_s0:lvm_state, lvm_sN:lvm_state,
     // assert lvm_s0.ok;
     assert ValidState(lvm_sM);
    
-  assert lvm_sM.ok;
-  assert lvm_b0.tl == lvm_bM;
+    assert lvm_sM.ok;
+    assert lvm_b0.tl == lvm_bM;
 
-  assert ValidState(lvm_sM);
-  assert evalCode_lax(lvm_cM, lvm_s0, lvm_sM);
-  reveal_evalCodeOpaque();
+    assert ValidState(lvm_sM);
+    assert evalCode_lax(lvm_cM, lvm_s0, lvm_sM);
+    reveal_evalCodeOpaque();
 }
 
 function method{:opaque} lvm_code_SHL(dst:lvm_operand_opr,src:lvm_operand_opr,shiftAmt:lvm_operand_opr):(out:lvm_code)
@@ -430,11 +423,10 @@ lemma lvm_lemma_Shl(lvm_b0:lvm_codes, lvm_s0:lvm_state, lvm_sN:lvm_state,
   requires ValidOperand(lvm_s0,shiftAmt);
 
   requires OperandContents(lvm_s0,src).Int?;
-  requires OperandContents(lvm_s0,dst).Int?;
+  // requires OperandContents(lvm_s0,dst).Int?;
   requires OperandContents(lvm_s0,shiftAmt).Int?;
   requires OperandContents(lvm_s0,src).itype.size*8 > OperandContents(lvm_s0,shiftAmt).val
   requires OperandContents(lvm_s0,shiftAmt).val > 0
-  requires OperandContents(lvm_s0,dst).itype.signed == OperandContents(lvm_s0,src).itype.signed
 // //   
   ensures  lvm_ensure(lvm_b0, lvm_bM, lvm_s0, lvm_sM, lvm_sN)
   ensures  lvm_get_ok(lvm_sM)
@@ -496,18 +488,18 @@ lemma lvm_lemma_Icmp(lvm_b0:lvm_codes, lvm_s0:lvm_state, lvm_sN:lvm_state,
   requires typesMatch(OperandContents(lvm_s0,op1),OperandContents(lvm_s0,op2));
   requires size == OperandContents(lvm_s0,op1).itype.size
 
-  ensures  lvm_ensure(lvm_b0, lvm_bM, lvm_s0, lvm_sM, lvm_sN)
-  ensures  lvm_get_ok(lvm_sM)
-  ensures  ValidOperand(lvm_sM,dst)
-  ensures  ValidOperand(lvm_sM,op1)
-  ensures  OperandContents(lvm_sM,dst).Int?;
-  ensures  OperandContents(lvm_sM,op1).Int?;
+  ensures lvm_ensure(lvm_b0, lvm_bM, lvm_s0, lvm_sM, lvm_sN)
+  ensures lvm_get_ok(lvm_sM)
+  ensures ValidOperand(lvm_sM,dst)
+  ensures ValidOperand(lvm_sM,op1)
+  ensures OperandContents(lvm_sM,dst).Int?;
+  ensures OperandContents(lvm_sM,op1).Int?;
   ensures OperandContents(lvm_s0,op1).itype == OperandContents(lvm_sM,op1).itype;
+  ensures !OperandContents(lvm_sM,dst).itype.signed
+  ensures OperandContents(lvm_sM,dst).itype.size == 1 
 
-  // ensures OperandContents(lvm_sM,dst).itype.size == OperandContents(lvm_sM,src).itype.size 
-  // ensures OperandContents(lvm_sM,dst).itype.signed == OperandContents(lvm_sM,src).itype.signed
   ensures OperandContents(lvm_sM, dst) == evalICMP(cond,size,OperandContents(lvm_s0,op1),OperandContents(lvm_s0,op2));
-  ensures  lvm_state_eq(lvm_sM, lvm_update_ok(lvm_sM, lvm_update_all( lvm_sM, lvm_s0)))
+  ensures lvm_state_eq(lvm_sM, lvm_update_ok(lvm_sM, lvm_update_all( lvm_sM, lvm_s0)))
   ensures forall d :: ValidOperand(lvm_s0,d) && d != dst ==> ValidOperand(lvm_sM,d) && OperandContents(lvm_s0,d) == OperandContents(lvm_sM,d)
   ensures StateNext(lvm_s0,lvm_sM)
 
@@ -568,13 +560,11 @@ lemma lvm_lemma_Empty(lvm_b0:lvm_codes, lvm_s0:lvm_state, lvm_sN:lvm_state)
     assert forall r :: r == lvm_s0 ==> eval_code(lvm_b0.hd,lvm_s0,r);
     assert evalCode_lax(Block(lvm_b0), lvm_s0, lvm_sN);
 
-
     // lvm_sM := lvm_lemma_empty(lvm_s0,lvm_sN);
     ghost var lvm_ltmp1, lvm_cM:lvm_code, lvm_ltmp2 := lvm_lemma_block(lvm_b0, lvm_s0, lvm_sN);
     lvm_sM := lvm_ltmp1;
     lvm_bM := lvm_ltmp2;
     var lvm_b1:lvm_codes := lvm_get_block(lvm_cM);
-    // assert evalCode_lax(lvm_Block(lvm_CNil()), lvm_s0, lvm_sM, o);
 
     lvm_sM := lvm_lemma_empty(lvm_s0, lvm_sM);
     assert ValidState(lvm_sM);
